src/Assembly/Wordize.v
@@ -4,6 +4,7 @@ Require Import Compare_dec Omega.
 Require Import FunctionalExtensionality ProofIrrelevance.
 Require Import QhasmUtil QhasmEvalCommon.
 Require Import WordizeUtil Bounds Vectorize List.
+Require Import NArithRing.
 
 Import EvalUtil ListNotations.
 
@@ -16,22 +17,19 @@ Coercion ind : bool >-> N.
 
 Section ToWord.
   Lemma wordize_plus: forall {n} (x y: word n),
-    (&x + &y)%N =
-      if (overflows n (&x + &y)%N)
-      then (& (x ^+ y) + Npow2 n)%N
-      else (& (x ^+ y)).
-  Proof. Admitted.
+      (&x + &y < Npow2 n)%N
+    -> (&x + &y)%N = & (x ^+ y).
+  Proof.
+  Admitted.
 
   Lemma wordize_awc: forall {n} (x y: word n) (c: bool),
-    (&x + &y + c)%N =
-      if (overflows n (&x + &y + c)%N)
-      then (&(addWithCarry x y c) + Npow2 n)%N
-      else (&(addWithCarry x y c)).
+      (&x + &y + c < Npow2 n)%N
+    -> (&x + &y + c)%N = &(addWithCarry x y c).
   Proof. Admitted.
 
-  Lemma wordize_mult: forall {n} (x y: word n) (b: N),
-    (&x * &y)%N = (&(x ^* y) +
-      &((EvalUtil.highBits (n/2) x) ^* (EvalUtil.highBits (n/2) y)) * Npow2 n)%N.
+  Lemma wordize_mult: forall {n} (x y: word n),
+      (&x * &y < Npow2 n)%N
+    -> (&x * &y)%N = &(x ^* y).
   Proof. intros. Admitted.
 
   Lemma wordize_shiftr: forall {n} (x: word n) (k: nat),
@@ -40,7 +38,32 @@ Section ToWord.
 
   Lemma conv_mask: forall {n} (x: word n) (k: nat),
     mask k x = x ^& (NToWord _ (N.ones (N.of_nat k))).
-  Proof. Admitted.
+  Proof.
+    intros.
+    apply NToWord_equal.
+    rewrite <- (Nat2N.id k).
+    rewrite mask_spec.
+    apply N.bits_inj_iff; unfold N.eqf; intro m.
+    rewrite N.land_spec.
+    repeat rewrite wordToN_testbit.
+    rewrite <- (N2Nat.id m).
+    rewrite <- wordToN_wones.
+    induction n; shatter x; try abstract (simpl; intuition).
+    induction (N.to_nat m).
+
+    - rewrite wordToN_wones in *.
+      rewrite N2Nat.id in *; rewrite Nat2N.id in *.
+      induction (whd x);
+        repeat rewrite andb_true_l;
+        repeat rewrite andb_false_l;
+        try reflexivity.
+      rewrite <- (Nat2N.id 0) in *.
+      rewrite <- wordToN_testbit.
+      setoid_rewrite <- wordToN_testbit in IHn.
+      admit.
+
+    - admit.
+  Admitted.
 End ToWord.
 
 Definition wordeq {ins outs} (n: nat) (f: Curried N N ins outs) :=
@@ -53,30 +76,25 @@ Definition wordeq {ins outs} (n: nat) (f: Curried N N ins outs) :=
 
 Ltac wordize_iter :=
   repeat match goal with
-  | [ |- context[overflows ?n ?x] ] => destruct (overflows n x)
-  | [ |- context[& ?x + & ?y + ind ?b] ] => rewrite wordize_awc
-  | [ |- context[N.mul (& ?x) (& ?y)] ] => rewrite wordize_mult
-  | [ |- context[N.add (& ?x) (& ?y)] ] => rewrite wordize_plus
-  | [ |- context[N.land (& ?x) _] ] => rewrite <- mask_spec
-  | [ |- context[N.shiftr (& ?x) ?k] ] => rewrite (wordize_shiftr x k)
-  | [ |- _ = _ ] => reflexivity
+  | [ |- context[& ?x + & ?y + ind ?b] ] =>
+    find_bound_on x; find_bound_on y; rewrite wordize_awc
+  | [ |- context[N.mul (& ?x) (& ?y)] ] =>
+    find_bound_on x; find_bound_on y; erewrite wordize_mult'
+  | [ |- context[N.add (& ?x) (& ?y)] ] =>
+    find_bound_on x; find_bound_on y; erewrite wordize_plus'
+  | [ |- context[N.land (& ?x) _] ] =>
+    find_bound_on x; rewrite <- mask_spec
+  | [ |- context[N.shiftr (& ?x) ?k] ] =>
+    find_bound_on x; rewrite (wordize_shiftr x k)
   end.
 
 Ltac wordize_intro :=
   repeat eexists; intros; list_destruct; simpl.
 
-Ltac wordize_contra :=
-  match goal with
-  | [ H: (_ >= _)%N |- _ ] =>
-    unfold N.ge in H;
-      contradict H;
-      apply N.compare_lt_iff;
-      compute_bound
-  end.
-
 Ltac wordize :=
   wordize_intro;
   wordize_iter;
-  wordize_contra.
+  bound_compute;
+  try reflexivity.
 
 Close Scope nword_scope.
